Kraken.lean
@@ -27,3 +27,5 @@ import Kraken.MachineWP
 import Kraken.SepWP
 import Kraken.SepSpecs
 import Kraken.SepFrameProc
+import Kraken.X64.Examples.SepAluMem
+import Kraken.X64.Examples.SepDynamicStack
